Added properness properties of interp functions

src/ItreeIMPOutput.v
@@ -95,7 +95,7 @@ Inductive stmt : Type :=
 | Seq    (a b : stmt)            (* a ; b *)
 | If     (i : expr) (t e : stmt) (* if (i) then { t } else { e } *)
 | While  (t : expr) (b : stmt)   (* while (t) { b } *)
-| Output (e : expr)              (* output e *)
+| Output (str : string)              (* output e *)
 | Skip                           (* ; *)
 .
 
@@ -172,9 +172,6 @@ Import ImpNotations.
 Variant ImpState : Type -> Type :=
 | GetVar (x : var) : ImpState value
 | SetVar (x : var) (v : value) : ImpState unit.
- 
-Variant OutputE : Type -> Type :=
-| Out (o : value) : OutputE unit.
 
 (** We can now define the denotation of _Imp_ expressions and statements.  We
     parameterize the denotation by a universe of events [eff], of which
@@ -195,10 +192,6 @@ Section Denote.
       parameterize the denotation of _Imp_ by a larger universe of events [eff],
       of which [ImpState] is assumed to be a subevent. *)
 
-  Context {eff : Type -> Type}.
-  Context {HasImpState : ImpState  -< eff}.
-    Context {HasPrintE : OutputE  -< eff}.
-
   (** _Imp_ expressions are denoted as [itree eff value], where the returned
       value in the tree is the value computed by the expression.
       In the [Var] case, the [trigger] operator smoothly lifts a single event to
@@ -207,7 +200,7 @@ Section Denote.
       A constant (literal) is simply returned.
       Usual monadic notations are used in the other cases: we can [bind]
       recursive computations in the case of operators as one would expect. *)
-Fixpoint denote_expr (e : expr) : itree eff value :=
+Fixpoint denote_expr (e : expr) : itree (ImpState +' (writerE string)) value :=
     match e with
     | Var v     => trigger (GetVar v)
     | Lit n     => ret n
@@ -216,36 +209,10 @@ Fixpoint denote_expr (e : expr) : itree eff value :=
     | Mult a b  => l <- denote_expr a ;; r <- denote_expr b ;; ret (l * r)
     end.
 
-  (** We turn to the denotation of statements. As opposed to expressions,
-      statements do not return any value: their semantic domain is therefore
-      [itree eff unit]. The most interesting construct is, naturally, [while].
+  
 
-      To define its meaning, we make use of the [iter] combinator provided by
-      the [itree] library:
-
-      [iter : (A -> itree E (A + B)) -> A -> itree E B].
-
-      The combinator takes as argument the body of the loop, i.e. a function
-      that maps inputs of type [A], the accumulator, to an [itree] computing
-      either a new [A] that can be fed back to the loop, or a return value of
-      type [B]. The combinator builds the fixpoint of the body, hiding away the
-      [A] argument from the return type.
-
-      Compared to the [mrec] and [rec] combinators introduced in
-      [Introduction.v], [iter] is more restricted in that it naturally
-      represents tail recursive functions.  It, however, enjoys a rich equational
-      theory: its addition grants the type of _continuation trees_ (named
-      [ktree]s in the library), a structure of _traced monoidal category_.
-
-      We use [loop] to first build a new combinator [while].
-      The accumulator degenerates to a single [unit] value indicating
-      whether we entered the body of the while loop or not. Since the
-      the operation does not return any value, the return type is also
-      taken to be [unit].
-      That is, the right tag [inr tt] says to exit the loop,
-      while the [inl tt] says to continue. *)
-
-  Definition while (step : itree eff (unit + unit)) : itree eff unit :=
+  Definition while (step : itree (ImpState +' (writerE string)) (unit + unit)) : 
+    itree (ImpState +' (writerE string)) unit :=
     iter (C := Kleisli _) (fun _ => step) tt.
 
   (** Casting values into [bool]:  [0] corresponds to [false] and any nonzero
@@ -256,7 +223,7 @@ Fixpoint denote_expr (e : expr) : itree eff value :=
       straightforward, except for [While], which uses our new [while] combinator
       over the computation that evaluates the conditional, and then the body if
       the former was true.  *)
-  Fixpoint denote_imp (s : stmt) : itree eff unit :=
+  Fixpoint denote_imp (s : stmt) : itree (ImpState +' (writerE string)) unit :=
     match s with
     | Assign x e =>  v <- denote_expr e ;; trigger (SetVar x v)
     | Seq a b    =>  denote_imp a ;; denote_imp b
@@ -269,431 +236,11 @@ Fixpoint denote_expr (e : expr) : itree eff value :=
 	           if is_true v
              then denote_imp b ;; ret (inl tt)
              else ret (inr tt))
-    | Output s =>  v<- denote_expr s;; trigger (Out v)
+    | Output str =>  tell str
     | Skip => ret tt
     end.
 
-    Fixpoint fold_constants_expr (a : expr) : expr :=
-      match a with
-      | Var x => Var x
-      | Lit n => Lit n
-      | Plus a1 a2 =>
-        match (fold_constants_expr a1,
-               fold_constants_expr a2)
-        with
-        | (Lit n1, Lit n2) => Lit (n1 + n2)
-        | (a1', a2') => Plus a1' a2'
-        end
-      | Minus a1 a2 =>
-        match (fold_constants_expr a1,
-               fold_constants_expr a2)
-        with
-        | (Lit n1, Lit n2) => Lit (n1 - n2)
-        | (a1', a2') => Minus a1' a2'
-        end
-      | Mult a1 a2 =>
-        match (fold_constants_expr a1,
-               fold_constants_expr a2)
-        with
-        | (Lit n1, Lit n2) => Lit (n1 * n2)
-        | (a1', a2') => Mult a1' a2'
-        end
-      end.
-    
-    Fixpoint fold_constants_stmt (s : stmt) : stmt :=
-      match s with
-      | Assign x e => Assign x (fold_constants_expr e)
-      | Seq s1 s2 => Seq (fold_constants_stmt s1) (fold_constants_stmt s2)
-      | If e s1 s2 => match fold_constants_expr e with
-                      | Lit 0 => fold_constants_stmt s2
-                      | Lit _ => fold_constants_stmt s1
-                      | e' => If e' (fold_constants_stmt s1) (fold_constants_stmt s2)
-                      end
-      | While e s => match fold_constants_expr e with
-                     | Lit 0 => Skip
-                     | Lit (S x) => While (Lit (S x)) (fold_constants_stmt s)
-                     | e' => While e' (fold_constants_stmt s)
-                     end
-      | Output e => Output (fold_constants_expr e)
-      | Skip => Skip
-      end.
-    
-    Theorem denote_imp_fold_constants_expr : forall e,
-        denote_expr  (fold_constants_expr e) ≅ denote_expr e.
-    Proof.
-      intros e; induction e; try reflexivity.
-      all: cbn; setoid_rewrite <- IHe1; setoid_rewrite <- IHe2.
-      all: destruct (fold_constants_expr e1) eqn:Eq1, (fold_constants_expr e2) eqn:Eq2.
-      all: cbn; try reflexivity.
-      all: now rewrite ?bind_ret_l.
-    Qed.
-    
-    Ltac bind := eapply eq_itree_clo_bind; [reflexivity | intros ? ? <-].
-    
-    (* This is what tripped me: without this instance, the rewrite marked as "HERE" in the proof below fails, forcing you to work around awkwardly otherwise *)
-    #[global] Instance missing_iter_instance {E R I}:
-      Proper (pointwise_relation I (eq_itree eq) ==> eq ==> eq_itree eq) (@ITree.iter E R I).
-    Proof.  
-      repeat intro.
-      subst. eapply eq_itree_iter. intros ?? <-. apply H.
-    Qed.
 
-    #[global] Instance missing_iter_instance' {E R I}:
-      Proper (pointwise_relation I (eutt eq) ==> eq ==> eutt eq) (@ITree.iter E R I).
-    Proof.  
-      repeat intro.
-      subst. eapply eutt_iter' with (RI := eq).
-      intros ?? <-. rewrite H. all: reflexivity.
-    Qed.
-    
-    Theorem denote_imp_fold_constants_stmt : forall s,
-        denote_imp  (fold_constants_stmt s) ≅ denote_imp s.
-    Proof.
-      intros s; induction s.
-      - cbn; now rewrite denote_imp_fold_constants_expr.
-      - cbn. now setoid_rewrite IHs1; setoid_rewrite IHs2.
-      - cbn.
-        rewrite <- (denote_imp_fold_constants_expr i).
-        destruct (fold_constants_expr i) eqn:eqi.
-        all: cbn.
-        all: try bind.
-        all: try now case is_true; eauto.
-        destruct v; subst; rewrite bind_ret_l.
-        now cbn; rewrite IHs2.
-        now cbn; rewrite IHs1.
-      - assert (BASE_CASE: forall (t : expr),
-                   denote_imp  (WHILE (fold_constants_expr t) DO (fold_constants_stmt s)) ≅
-                   denote_imp (WHILE t DO s)
-               ).
-        { clear t; intros t.
-          cbn.
-          eapply eq_itree_iter; intros ?? <-.
-          try (rewrite denote_imp_fold_constants_expr; bind).
-          case is_true; try reflexivity.
-          try now rewrite IHs.
-        }
-        cbn.
-        destruct (fold_constants_expr t) eqn:eqt; [| destruct v |..];
-          try (rewrite <- eqt; apply BASE_CASE).
-        cbn.
-        unfold while.
-        (* HERE *)
-        setoid_rewrite <- (denote_imp_fold_constants_expr t).
-        rewrite eqt.
-        cbn.
-        rewrite unfold_iter_ktree.
-        rewrite ? bind_ret_l.
-        now cbn; rewrite ? bind_ret_l.
-        - cbn. rewrite denote_imp_fold_constants_expr. reflexivity.
-      - reflexivity.
-    Qed.
-
-Theorem denote_imp_fold_constants_expr_weak : forall e,
-    denote_expr (fold_constants_expr e) ≈ denote_expr e.  
-Proof. 
-  intros.
-  induction e.
-  - simpl. reflexivity.
-  - simpl. reflexivity.
-  -  unfold denote_expr. fold denote_expr. rewrite <- IHe1. 
-    setoid_rewrite <- IHe2. simpl. destruct (fold_constants_expr e1) eqn:He1; 
-      destruct (fold_constants_expr e2) eqn:He2; simpl; try reflexivity. rewrite bind_ret_l. rewrite bind_ret_l. reflexivity.
-  - unfold denote_expr. fold denote_expr. rewrite <- IHe1.
-    setoid_rewrite <- IHe2. simpl. destruct (fold_constants_expr e1) eqn:He1; 
-      destruct (fold_constants_expr e2) eqn:He2; simpl; try reflexivity. rewrite bind_ret_l. rewrite bind_ret_l. reflexivity.
-  - unfold denote_expr. fold denote_expr. rewrite <- IHe1.
-    setoid_rewrite <- IHe2. simpl. destruct (fold_constants_expr e1) eqn:He1; 
-      destruct (fold_constants_expr e2) eqn:He2; simpl; try reflexivity. rewrite bind_ret_l. rewrite bind_ret_l. reflexivity.
-Qed.
-
-
-Theorem denote_imp_fold_constants_stmt_weak : forall s,
-    denote_imp (fold_constants_stmt s) ≈ denote_imp s.
-Proof.
-  induction s. intros. 
-  - simpl. rewrite denote_imp_fold_constants_expr_weak. reflexivity.
-  - simpl. rewrite IHs1. setoid_rewrite IHs2. reflexivity.
-  - simpl.
-     rewrite <- denote_imp_fold_constants_expr_weak.
-    destruct (fold_constants_expr i). 
-    + apply eqit_bind. reflexivity. 
-      red.
-      simpl. intros. destruct a; simpl; try reflexivity.
-      rewrite IHs2. reflexivity.
-      rewrite IHs1. reflexivity.
-    + destruct v.
-      * simpl. rewrite bind_ret_l. simpl. rewrite IHs2. reflexivity.
-      * simpl. rewrite bind_ret_l. simpl. rewrite IHs1. reflexivity.
-    + apply eqit_bind. reflexivity. 
-      red.
-      simpl. intros. destruct a; simpl; try reflexivity.
-      rewrite IHs2. reflexivity.
-      rewrite IHs1. reflexivity.
-    + apply eqit_bind. reflexivity. 
-      red.
-      simpl. intros. destruct a; simpl; try reflexivity.
-      rewrite IHs2. reflexivity.
-      rewrite IHs1. reflexivity.
-    + apply eqit_bind. reflexivity.
-        red.
-        simpl. intros. destruct a; simpl; try reflexivity.
-        rewrite IHs2. reflexivity.
-        rewrite IHs1. reflexivity.
-  - assert (BASE_CASE: forall (t : expr),
-    denote_imp  (WHILE (fold_constants_expr t) DO (fold_constants_stmt s)) ≈
-    denote_imp (WHILE t DO s)
-).
-{ intros.
-simpl. apply eutt_iter' with (RI := eq).
-intros _ _ []. apply eutt_clo_bind with (UU := eq); try reflexivity.
-apply denote_imp_fold_constants_expr_weak.
-intros. subst. destruct u2. simpl. reflexivity. simpl. rewrite IHs. reflexivity. reflexivity. 
-}
-cbn. destruct (fold_constants_expr t) eqn:eqt; [| destruct v |..].
-+ rewrite <- eqt. apply BASE_CASE.
-+ unfold while. unfold while. unfold iter. unfold Iter_Kleisli. unfold Basics.iter. unfold MonadIter_itree.
-  simpl.
-  rewrite unfold_iter. rewrite bind_bind.
-  rewrite <- denote_imp_fold_constants_expr_weak. rewrite eqt. simpl.
-  rewrite bind_ret_l. simpl. rewrite bind_ret_l. reflexivity.
-+ rewrite <- eqt. apply BASE_CASE.
-+ rewrite <- eqt. apply BASE_CASE.
-+ rewrite <- eqt. apply BASE_CASE.
-+ rewrite <- eqt. apply BASE_CASE. 
-- simpl. rewrite denote_imp_fold_constants_expr_weak. reflexivity.
-  - simpl. reflexivity.
-    Qed. 
-  
- 
-Theorem CAsgn_congruence : forall x a a',
-    denote_expr a  ≅ denote_expr a' ->
-    denote_imp (Assign x a) ≅ denote_imp (Assign x a').
-  Proof.  
-    intros x a a' Heqv.  
-    simpl. rewrite Heqv. reflexivity. Qed.
-
-Theorem CAsgn_congruence_weak : forall x a a',
-    denote_expr a  ≈ denote_expr a' ->
-    denote_imp (Assign x a) ≈ denote_imp (Assign x a').
-  Proof.  
-    intros x a a' Heqv.  
-    simpl. rewrite Heqv. reflexivity. Qed.
-
-Theorem CSeq_congruence : forall c1 c1' c2 c2',
-    denote_imp c1 ≅ denote_imp c1' ->
-    denote_imp c2 ≅ denote_imp c2' ->
-    denote_imp (Seq c1 c2) ≅ denote_imp (Seq c1' c2').
-  Proof.
-    intros c1 c1' c2 c2' Heqc1 Heqc2.
-    simpl. apply eqit_bind.
-    - rewrite Heqc1. reflexivity.
-    - intros. setoid_rewrite Heqc2. reflexivity. Qed.
-
-  Theorem CSeq_congruence_weak : forall c1 c1' c2 c2',
-    denote_imp c1 ≈ denote_imp c1' ->
-    denote_imp c2 ≈ denote_imp c2' ->
-    denote_imp (Seq c1 c2) ≈ denote_imp (Seq c1' c2').
-  Proof.
-    intros c1 c1' c2 c2' Heqc1 Heqc2.
-    simpl. apply eqit_bind.
-    - rewrite Heqc1. reflexivity.
-    - intros. setoid_rewrite Heqc2. reflexivity. Qed.
-
-  Theorem CIf_congruence : forall i i' t t' e e',
-      denote_expr i ≅ denote_expr i' ->
-      denote_imp t ≅ denote_imp t' ->
-      denote_imp e ≅ denote_imp e' ->
-      denote_imp (If i t e) ≅ denote_imp (If i' t' e').
-  Proof.
-    intros i i' t t' e e' Heqi Heqt Heqe.
-    simpl. rewrite Heqi.
-    apply eqit_bind; [ reflexivity | ].
-    intros []. case is_true; auto. 
-    simpl. rewrite Heqt. reflexivity. 
-    
-    Qed.
-
-  Theorem CIf_congruence_weak : forall i i' t t' e e',
-      denote_expr i ≈ denote_expr i' ->
-      denote_imp t ≈ denote_imp t' ->
-      denote_imp e ≈ denote_imp e' ->
-      denote_imp (If i t e) ≈ denote_imp (If i' t' e').
-  Proof.
-    intros i i' t t' e e' Heqi Heqt Heqe.
-    simpl. rewrite Heqi.
-    apply eqit_bind; [ reflexivity | ].
-    intros []. case is_true; auto. 
-    simpl. rewrite Heqt. reflexivity. 
-    
-    Qed.
-
-  Theorem CWhile_congruence : forall t t' b b',
-      denote_expr t ≅ denote_expr t' ->
-      denote_imp b ≅ denote_imp b' ->
-      denote_imp (While t b) ≅ denote_imp (While t' b').
-
-
-  Proof.
-    intros t t' b b' Heqt Heqb.
-    simpl. unfold while.
-    eapply eq_itree_iter; intros ?? <-.
-    apply eqit_bind.
-    rewrite Heqt. reflexivity.
-
-    intros []. case is_true; auto.
-    simpl. rewrite Heqb. reflexivity. reflexivity.
-    simpl. rewrite Heqb. reflexivity.
-    Qed.
-
- 
-  Theorem CWhile_congruence_weak : forall t t' b b',
-      denote_expr t ≈ denote_expr t' ->
-      denote_imp b ≈ denote_imp b' ->
-      denote_imp (While t b) ≈ denote_imp (While t' b').
-  Proof.
-    intros t t' b b' Heqt Heqb.
-    simpl. unfold while.
-    apply eutt_iter' with (RI := eq). intros _ _ []. apply eutt_clo_bind with (UU := eq); try reflexivity.
-    assumption. intros. subst. destruct u2. simpl. reflexivity. simpl. rewrite Heqb. reflexivity. reflexivity.
-    Qed.
-    
-Theorem COut_congruence : forall e e',
-    denote_expr e ≅ denote_expr e' ->
-    denote_imp (Output e) ≅ denote_imp (Output e').
-  Proof.
-    intros e e' Heqe. simpl. rewrite Heqe. reflexivity. Qed.
-
-
-
-    Theorem denote_imp_fold_constants_stmt_with_congruence : forall s,
-        denote_imp (fold_constants_stmt s) ≅ denote_imp s.
-    Proof.
-      intros s; induction s.
-      - apply CAsgn_congruence. apply denote_imp_fold_constants_expr.
-      -  unfold fold_constants_stmt. fold fold_constants_stmt.
-         apply CSeq_congruence; try reflexivity.
-         apply IHs1. apply IHs2.
-      - unfold fold_constants_stmt. 
-        fold fold_constants_stmt.
-        unfold denote_imp. fold denote_imp.
-        rewrite <- (denote_imp_fold_constants_expr i).
-        destruct (fold_constants_expr i) eqn:eqi.
-        + apply CIf_congruence; try reflexivity. 
-          apply IHs1. apply IHs2.
-        + destruct v.
-          * simpl. rewrite bind_ret_l. simpl.  
-            apply IHs2.
-          * simpl. rewrite bind_ret_l. simpl.  
-            apply IHs1.
-        + apply CIf_congruence; try reflexivity.
-          apply IHs1. apply IHs2.
-        + apply CIf_congruence; try reflexivity.
-          apply IHs1. apply IHs2.
-        + apply CIf_congruence; try reflexivity.
-          apply IHs1. apply IHs2.
-      - unfold fold_constants_stmt. fold fold_constants_stmt.
-        unfold denote_imp. fold denote_imp.
-        unfold while.
-        setoid_rewrite <- (denote_imp_fold_constants_expr t).
-          destruct (fold_constants_expr t) eqn:eqt; 
-          try apply CWhile_congruence; try reflexivity; try apply IHs.
-          * destruct v. simpl.
-            unfold iter. unfold Iter_Kleisli. unfold Basics.iter. unfold MonadIter_itree.
-            rewrite unfold_iter. rewrite bind_bind.
-            
-            rewrite bind_ret_l. simpl. rewrite bind_ret_l. reflexivity.
-            apply CWhile_congruence; try reflexivity. apply IHs.
-    - simpl. rewrite denote_imp_fold_constants_expr. reflexivity.
-      - reflexivity.
-    Qed.
-
-    Theorem denote_imp_fold_constants_stmt_with_congruence_weak : forall s,
-        denote_imp (fold_constants_stmt s) ≈ denote_imp s.
-    Proof.
-      intros s; induction s.
-      - apply CAsgn_congruence_weak. apply denote_imp_fold_constants_expr_weak.
-      -  unfold fold_constants_stmt. fold fold_constants_stmt.
-         apply CSeq_congruence_weak; try reflexivity.
-         apply IHs1. apply IHs2.
-      - unfold fold_constants_stmt. 
-        fold fold_constants_stmt.
-        unfold denote_imp. fold denote_imp.
-        rewrite <- (denote_imp_fold_constants_expr_weak i).
-        destruct (fold_constants_expr i) eqn:eqi.
-        + apply CIf_congruence_weak; try reflexivity. 
-          apply IHs1. apply IHs2.
-        + destruct v.
-          * simpl. rewrite bind_ret_l. simpl.  
-            apply IHs2.
-          * simpl. rewrite bind_ret_l. simpl.  
-            apply IHs1.
-        + apply CIf_congruence_weak; try reflexivity.
-          apply IHs1. apply IHs2.
-        + apply CIf_congruence_weak; try reflexivity.
-          apply IHs1. apply IHs2.
-        + apply CIf_congruence_weak; try reflexivity.
-          apply IHs1. apply IHs2.
-      - unfold fold_constants_stmt. fold fold_constants_stmt.
-        unfold denote_imp. fold denote_imp.
-        unfold while.
-         
-        setoid_rewrite <- (denote_imp_fold_constants_expr_weak t).
-          destruct (fold_constants_expr t) eqn:eqt; 
-          try apply CWhile_congruence_weak; try reflexivity; try apply IHs.
-          * destruct v. simpl. rewrite unfold_iter_ktree. rewrite ? bind_ret_l. 
-            now cbn; rewrite ? bind_ret_l.
-            apply CWhile_congruence_weak; try reflexivity. apply IHs.
-    - simpl. rewrite denote_imp_fold_constants_expr_weak. reflexivity. 
-      - reflexivity.
-        Qed.
-        
-
-Example while_different_print_not_equivalent: 
-  (denote_imp (While (Lit 1) (Output (Lit 1))) ≈ 
-  denote_imp (While (Lit 1) (Output (Lit 2)))) -> False.
-Proof. Admitted.  
-End Denote.
-
-(* ========================================================================== *)
-(** ** Equivalence of Imp programs *)
-
-(** Two _Imp_ programs are equivalent if they denote the same tree.  *)
-
-
-(** We provide an _ITree event handler_ to interpret away [ImpState] events.  We
-    use an _environment event_ to do so, modeling the environment as a
-    0-initialized map from strings to values.  Recall from [Introduction.v] that
-    a _handler_ for the events [ImpState] is a function of type [forall R, ImpState R
-    -> M R] for some monad [M].  Here we take for our monad the special case of
-    [M = itree E] for some universe of events [E] required to contain the
-    environment events [mapE] provided by the library. It comes with an event
-    interpreter [interp_map] that yields a computation in the state monad.  *)
-    
-Definition handle_ImpState {E: Type -> Type} `{mapE var 0 -< E}: ImpState ~> itree E :=
-  fun _ e =>
-    match e with
-    | GetVar x => lookup_def x
-    | SetVar x v => insert x v
-    end.
-
-Definition handle_OutputE {E : Type -> Type} `{mapE var 0 -< E}: OutputE ~> itree E :=
-      fun _ e =>
-        match e with
-        | Out s => ret tt
-        end.
-Check handle_ImpState.
-Check handle_OutputE.
-
- 
-
-(** We can now define an evaluator for our statements.
-   To do so, we first denote them, leading to an [itree ImpState unit].
-   We then [interp]ret [ImpState] into [mapE] using [handle_ImpState], leading to
-   an [itree (mapE var value) unit].
-   Finally, [interp_map] interprets the latter [itree] into the state monad,
-   resulting in an [itree] free of any event, but returning the final
-   _Imp_ env.
- *)
 
 From ITree Require Import
      Events.MapDefault.
@@ -703,122 +250,458 @@ From ExtLib Require Import
      Core.RelDec
      Structures.Maps
      Data.Map.FMapAList.
-
-Definition env := alist var value.
-
-
-(** We now concretely implement this environment using ExtLib's finite maps. *)
+     Definition env := alist var value.
 
 
-(** Finally, we can define an evaluator for our statements.
-   To do so, we first denote them, leading to an [itree ImpState unit].
-   We then [interp]ret [ImpState] into [mapE] using [handle_ImpState], leading to
-   an [itree (mapE var value) unit].
-   Finally, [interp_map] interprets the latter [itree] into the state monad,
-   resulting in an [itree] free of any event, but returning the final
-   _Imp_ env.
- *)
-(* SAZ: would rather write something like the following:
- h : E ~> M A
- h' : F[void1] ~> M A
-forall eff, {pf:E -< eff == F[E]} (t : itree eff A)
-        interp pf h h' t : M A
-*)
-  Section Example_Fact.
+Definition empty : env := nil.
 
-  (** We briefly illustrate the language by writing the traditional factorial.
-      example.  *)
+Definition handle_ImpState: ImpState ~> itree (mapE var 0) :=
+  fun _ e =>
+    match e with
+    | GetVar x => lookup_def x
+    | SetVar x v => insert x v
+    end.
 
-  Open Scope expr_scope.
-  Open Scope stmt_scope.
-  Variable input: var.
-  Variable output: var.
-
-  Definition fact (n:nat): stmt :=
-    input ← n;;;
-    output ← 1;;;
-    WHILE input
-    DO output ← output * input;;;
-       Output output;;;
-       input  ← input - 1.
-
-  (** We have given _a_ notion of denotation to [fact 6] via [denote_imp].
-      However, this is naturally not actually runnable yet, since it contains
-      uninterpreted [ImpState] events.  We therefore now need to _handle_ the
-      events contained in the trees, i.e. give a concrete interpretation of the
-      environment.  *)
-
-
-(*
-Compute denote_imp (fact 8).
-Variable E: Type -> Type.
-Check stateT env (itree E) (list nat).
-Check handle_ImpState.
-
-Definition interp_imp  {E A} (t : itree ((ImpState +' OutputE) +' E) A) : stateT env (itree E) A :=
-  let t' := interp (bimap  handle_ImpState  (id_ E)) t in
-  interp_map t'.
-
-
-Definition eval_imp (s: stmt) : itree void1 (env * unit) :=
-  interp_imp (denote_imp s) empty.
-
-(** Equipped with this evaluator, we can now compute.
-    Naturally since Coq is total, we cannot do it directly inside of it.
-    We can either rely on extraction, or use some fuel.
- *)
-
-
-(* ========================================================================== *)
-Section InterpImpProperties.
-  (** We can lift the underlying equational theory on [itree]s to include new
-      equations for working with [interp_imp].
-
-      In particular, we have:
-         - [interp_imp] respects [≈]
-         - [interp_imp] commutes with [bind].
-
-      We could justify more equations than just the ones below.  For instance,
-      _Imp_ programs also respect a coarser notation of equivalence for the
-      [env] state.  We exploit this possibility to implement optimzations
-      at the _Asm_ level (see AsmOptimizations.v).
-   *)
-
-  
-    Context {E': Type -> Type}.
-  Notation E := (ImpState +' E').
-
-  (** This interpreter is compatible with the equivalence-up-to-tau. *)
-  Global Instance eutt_interp_imp {R}:
-    Proper (@eutt E R R eq ==> eq ==> @eutt E' (prod (env) R) (prod _ R) eq)
-           interp_imp.
+    Typeclasses eauto := 5.
+    Example while_different_print_not_equivalent: 
+    (denote_imp (While (Lit 1) (Output "s")) ≈ 
+    denote_imp (While (Lit 1) (Output "n"))) -> False.
   Proof.
-    repeat intro.
-    unfold interp_imp.
-    unfold interp_map.
-    rewrite H0. eapply eutt_interp_state_eq; auto.
-    rewrite H. reflexivity.
-  Qed.
+    Admitted. 
 
-  (** [interp_imp] commutes with [bind]. *)
-  Lemma interp_imp_bind: forall {R S} (t: itree E R) (k: R -> itree E S) (g : env),
-      (interp_imp (ITree.bind t k) g)
-    ≅ (ITree.bind (interp_imp t g) (fun '(g',  x) => interp_imp (k x) g')).
-  Proof.
-    intros.
-    unfold interp_imp.
-    unfold interp_map.
-    repeat rewrite interp_bind.
-    repeat rewrite interp_state_bind.
-    apply eqit_bind; [ reflexivity | ].
-    red. intros.
-    destruct a as [g'  x].
-    simpl.
-    reflexivity.
-  Qed.
+End Denote.
+Check denote_imp. 
+
+Definition interp_imp_implicit_E {E} (t : itree (ImpState +' E) unit) :
+  stateT (env) (itree E) unit :=
+   interp_map (interp (bimap handle_ImpState (id_ E)) t).
+
+Definition interp_imp_state:= @interp_imp_implicit_E (writerE string).
+Check interp_imp_state.
+
+Definition eval_imp_state (s: stmt) : itree (writerE string) (env * unit) :=
+  interp_imp_state (denote_imp s) empty.
+
+Variant voidE : Type -> Type :=  .
+
+Check interp (@handle_writer_list string voidE) .
+
+Definition interp_output (t : itree (writerE string) (env * unit)) :=
+  interp (@handle_writer_list string voidE) t.
+
+Definition eval_imp (s: stmt)  :=
+  interp_output (interp_imp_state (denote_imp s) empty) nil.
+
+Section Example_Fact.
+Open Scope expr_scope.
+Open Scope stmt_scope.
+Variable input: var.
+Variable output: var.
+
+Definition fact (n:nat): stmt :=
+  input ← n;;;
+  output ← 1;;;
+  WHILE input
+  DO output ← output * input;;;
+    Output "some statement";;;
+     input  ← input - 1.
+End Example_Fact.
+
+Compute (burn 2000 (eval_imp (fact "input" "output" 9))).
+
+
+Global Instance eutt_interp_imp_state:
+Proper (@eutt (ImpState +' (writerE string)) unit unit eq ==> eq ==> @eutt (writerE string) (prod (env) unit) (prod _ unit) eq)
+  interp_imp_state.
+Proof.
+  repeat intro.
+  subst.
+  unfold interp_imp_state.
+  unfold interp_imp_implicit_E.
+  unfold interp_map. rewrite H. reflexivity. Qed.
   
+Check @eutt (writerE string) (prod (env) unit) (prod _ unit) .
+Check interp_imp_state.
+Global Instance eutt_interp_output:
+  Proper (@eutt (writerE string) (env * unit) (env * unit) eq ==>
+          eq ==>
+          @eutt voidE (prod (list string) (env * unit)) (prod _ (env * unit)) eq)
+  interp_output.
+Proof.
+  repeat intro.
+  subst.
+  unfold interp_output.
+  rewrite H. reflexivity. Qed.
 
-End InterpImpProperties.
-*)
 
-(** We now turn to our target language, in file [Asm].v *)
+Fixpoint fold_constants_expr (a : expr) : expr :=
+          match a with
+          | Var x => Var x
+          | Lit n => Lit n
+          | Plus a1 a2 =>
+            match (fold_constants_expr a1,
+                   fold_constants_expr a2)
+            with
+            | (Lit n1, Lit n2) => Lit (n1 + n2)
+            | (a1', a2') => Plus a1' a2'
+            end
+          | Minus a1 a2 =>
+            match (fold_constants_expr a1,
+                   fold_constants_expr a2)
+            with
+            | (Lit n1, Lit n2) => Lit (n1 - n2)
+            | (a1', a2') => Minus a1' a2'
+            end
+          | Mult a1 a2 =>
+            match (fold_constants_expr a1,
+                   fold_constants_expr a2)
+            with
+            | (Lit n1, Lit n2) => Lit (n1 * n2)
+            | (a1', a2') => Mult a1' a2'
+            end
+          end.
+        
+          Fixpoint fold_constants_stmt (s : stmt) : stmt :=
+            match s with
+            | Assign x e => Assign x (fold_constants_expr e)
+            | Seq s1 s2 => Seq (fold_constants_stmt s1) (fold_constants_stmt s2)
+            | If e s1 s2 => match fold_constants_expr e with
+                            | Lit 0 => fold_constants_stmt s2
+                            | Lit _ => fold_constants_stmt s1
+                            | e' => If e' (fold_constants_stmt s1) (fold_constants_stmt s2)
+                            end
+            | While e s => match fold_constants_expr e with
+                           | Lit 0 => Skip
+                           | Lit (S x) => While (Lit (S x)) (fold_constants_stmt s)
+                           | e' => While e' (fold_constants_stmt s)
+                           end
+            | Output e => Output e
+            | Skip => Skip
+            end.
+          
+Theorem denote_imp_fold_constants_expr : forall e,
+              denote_expr  (fold_constants_expr e) ≅ denote_expr e.
+Proof.
+            intros e; induction e; try reflexivity.
+            all: cbn; setoid_rewrite <- IHe1; setoid_rewrite <- IHe2.
+            all: destruct (fold_constants_expr e1) eqn:Eq1, (fold_constants_expr e2) eqn:Eq2.
+            all: cbn; try reflexivity.
+            all: now rewrite ?bind_ret_l.
+          Qed.
+          
+          Ltac bind := eapply eq_itree_clo_bind; [reflexivity | intros ? ? <-].
+          
+          (* This is what tripped me: without this instance, the rewrite marked as "HERE" in the proof below fails, forcing you to work around awkwardly otherwise *)
+          #[global] Instance missing_iter_instance {E R I}:
+            Proper (pointwise_relation I (eq_itree eq) ==> eq ==> eq_itree eq) (@ITree.iter E R I).
+          Proof.  
+            repeat intro.
+            subst. eapply eq_itree_iter. intros ?? <-. apply H.
+          Qed.
+      
+          #[global] Instance missing_iter_instance' {E R I}:
+            Proper (pointwise_relation I (eutt eq) ==> eq ==> eutt eq) (@ITree.iter E R I).
+          Proof.  
+            repeat intro.
+            subst. eapply eutt_iter' with (RI := eq).
+            intros ?? <-. rewrite H. all: reflexivity.
+          Qed.
+          
+          Theorem denote_imp_fold_constants_stmt : forall s,
+              denote_imp  (fold_constants_stmt s) ≅ denote_imp s.
+          Proof.
+            intros s; induction s.
+            - cbn; now rewrite denote_imp_fold_constants_expr.
+            - cbn. now setoid_rewrite IHs1; setoid_rewrite IHs2.
+            - cbn.
+              rewrite <- (denote_imp_fold_constants_expr i).
+              destruct (fold_constants_expr i) eqn:eqi.
+              all: cbn.
+              all: try bind.
+              all: try now case is_true; eauto.
+              destruct v; subst; rewrite bind_ret_l.
+              now cbn; rewrite IHs2.
+              now cbn; rewrite IHs1.
+            - assert (BASE_CASE: forall (t : expr),
+                         denote_imp  (WHILE (fold_constants_expr t) DO (fold_constants_stmt s)) ≅
+                         denote_imp (WHILE t DO s)
+                     ).
+              { clear t; intros t.
+                cbn.
+                eapply eq_itree_iter; intros ?? <-.
+                try (rewrite denote_imp_fold_constants_expr; bind).
+                case is_true; try reflexivity.
+                try now rewrite IHs.
+              }
+              cbn.
+              destruct (fold_constants_expr t) eqn:eqt; [| destruct v |..];
+            try (rewrite <- eqt; apply BASE_CASE).
+              unfold while.
+              (* HERE *)
+              setoid_rewrite <- (denote_imp_fold_constants_expr t).
+                rewrite eqt.
+          cbn.
+          rewrite unfold_iter_ktree.
+          rewrite ? bind_ret_l.
+          now cbn; rewrite ? bind_ret_l.
+  
+        - reflexivity.
+        - reflexivity. Qed.
+      
+      Theorem denote_imp_fold_constants_expr_weak : forall e,
+          denote_expr (fold_constants_expr e) ≈ denote_expr e.  
+      Proof. 
+        intros.
+        induction e.
+        - simpl. reflexivity.
+        - simpl. reflexivity.
+        -  unfold denote_expr. fold denote_expr. rewrite <- IHe1. 
+          setoid_rewrite <- IHe2. simpl. destruct (fold_constants_expr e1) eqn:He1; 
+            destruct (fold_constants_expr e2) eqn:He2; simpl; try reflexivity. rewrite bind_ret_l. rewrite bind_ret_l. reflexivity.
+        - unfold denote_expr. fold denote_expr. rewrite <- IHe1.
+          setoid_rewrite <- IHe2. simpl. destruct (fold_constants_expr e1) eqn:He1; 
+            destruct (fold_constants_expr e2) eqn:He2; simpl; try reflexivity. rewrite bind_ret_l. rewrite bind_ret_l. reflexivity.
+        - unfold denote_expr. fold denote_expr. rewrite <- IHe1.
+          setoid_rewrite <- IHe2. simpl. destruct (fold_constants_expr e1) eqn:He1; 
+            destruct (fold_constants_expr e2) eqn:He2; simpl; try reflexivity. rewrite bind_ret_l. rewrite bind_ret_l. reflexivity.
+      Qed.
+      
+      
+      Theorem denote_imp_fold_constants_stmt_weak : forall s,
+          denote_imp (fold_constants_stmt s) ≈ denote_imp s.
+      Proof.
+        induction s. intros. 
+        -  simpl. rewrite denote_imp_fold_constants_expr_weak. reflexivity.
+        - simpl. rewrite IHs1. setoid_rewrite IHs2. reflexivity.
+        - simpl.
+           rewrite <- denote_imp_fold_constants_expr_weak.
+          destruct (fold_constants_expr i). 
+          + apply eqit_bind. reflexivity. 
+            red.
+            simpl. intros. destruct a; simpl; try reflexivity.
+            rewrite IHs2. reflexivity.
+            rewrite IHs1. reflexivity.
+          + destruct v.
+            * simpl. rewrite bind_ret_l. simpl. rewrite IHs2. reflexivity.
+            * simpl. rewrite bind_ret_l. simpl. rewrite IHs1. reflexivity.
+          + apply eqit_bind. reflexivity. 
+            red.
+            simpl. intros. destruct a; simpl; try reflexivity.
+            rewrite IHs2. reflexivity.
+            rewrite IHs1. reflexivity.
+          + apply eqit_bind. reflexivity. 
+            red.
+            simpl. intros. destruct a; simpl; try reflexivity.
+            rewrite IHs2. reflexivity.
+            rewrite IHs1. reflexivity.
+          + apply eqit_bind. reflexivity.
+              red.
+              simpl. intros. destruct a; simpl; try reflexivity.
+              rewrite IHs2. reflexivity.
+              rewrite IHs1. reflexivity.
+        - assert (BASE_CASE: forall (t : expr),
+          denote_imp  (WHILE (fold_constants_expr t) DO (fold_constants_stmt s)) ≈
+          denote_imp (WHILE t DO s)
+      ).
+      { intros.
+      simpl. apply eutt_iter' with (RI := eq).
+      intros _ _ []. apply eutt_clo_bind with (UU := eq); try reflexivity.
+      apply denote_imp_fold_constants_expr_weak.
+      intros. subst. destruct u2. simpl. reflexivity. simpl. rewrite IHs. reflexivity. reflexivity. 
+      }
+      cbn. destruct (fold_constants_expr t) eqn:eqt; [| destruct v |..].
+      + rewrite <- eqt. apply BASE_CASE.
+      + unfold while. unfold while. unfold iter. unfold Iter_Kleisli. unfold Basics.iter. unfold MonadIter_itree.
+        simpl.
+        rewrite unfold_iter. rewrite bind_bind.
+        rewrite <- denote_imp_fold_constants_expr_weak. rewrite eqt. simpl.
+        rewrite bind_ret_l. simpl. rewrite bind_ret_l. reflexivity.
+      + rewrite <- eqt. apply BASE_CASE.
+      + rewrite <- eqt. apply BASE_CASE.
+      + rewrite <- eqt. apply BASE_CASE.
+      + rewrite <- eqt. apply BASE_CASE. 
+      - simpl. reflexivity.
+        - simpl. reflexivity.
+          Qed. 
+        
+       
+      Theorem CAsgn_congruence : forall x a a',
+          denote_expr a  ≅ denote_expr a' ->
+          denote_imp (Assign x a) ≅ denote_imp (Assign x a').
+        Proof.  
+          intros x a a' Heqv.  
+          simpl. rewrite Heqv. reflexivity. Qed.
+      
+      Theorem CAsgn_congruence_weak : forall x a a',
+          denote_expr a  ≈ denote_expr a' ->
+          denote_imp (Assign x a) ≈ denote_imp (Assign x a').
+        Proof.  
+          intros x a a' Heqv.  
+          simpl. rewrite Heqv. reflexivity. Qed.
+      
+      Theorem CSeq_congruence : forall c1 c1' c2 c2',
+          denote_imp c1 ≅ denote_imp c1' ->
+          denote_imp c2 ≅ denote_imp c2' ->
+          denote_imp (Seq c1 c2) ≅ denote_imp (Seq c1' c2').
+        Proof.
+          intros c1 c1' c2 c2' Heqc1 Heqc2.
+          simpl. apply eqit_bind.
+          - rewrite Heqc1. reflexivity.
+          - intros. setoid_rewrite Heqc2. reflexivity. Qed.
+      
+        Theorem CSeq_congruence_weak : forall c1 c1' c2 c2',
+          denote_imp c1 ≈ denote_imp c1' ->
+          denote_imp c2 ≈ denote_imp c2' ->
+          denote_imp (Seq c1 c2) ≈ denote_imp (Seq c1' c2').
+        Proof.
+          intros c1 c1' c2 c2' Heqc1 Heqc2.
+          simpl. apply eqit_bind.
+          - rewrite Heqc1. reflexivity.
+          - intros. setoid_rewrite Heqc2. reflexivity. Qed.
+      
+        Theorem CIf_congruence : forall i i' t t' e e',
+            denote_expr i ≅ denote_expr i' ->
+            denote_imp t ≅ denote_imp t' ->
+            denote_imp e ≅ denote_imp e' ->
+            denote_imp (If i t e) ≅ denote_imp (If i' t' e').
+        Proof.
+          intros i i' t t' e e' Heqi Heqt Heqe.
+          simpl. rewrite Heqi.
+          apply eqit_bind; [ reflexivity | ].
+          intros []. case is_true; auto. 
+          simpl. rewrite Heqt. reflexivity. 
+          
+          Qed.
+      
+        Theorem CIf_congruence_weak : forall i i' t t' e e',
+            denote_expr i ≈ denote_expr i' ->
+            denote_imp t ≈ denote_imp t' ->
+            denote_imp e ≈ denote_imp e' ->
+            denote_imp (If i t e) ≈ denote_imp (If i' t' e').
+        Proof.
+          intros i i' t t' e e' Heqi Heqt Heqe.
+          simpl. rewrite Heqi.
+          apply eqit_bind; [ reflexivity | ].
+          intros []. case is_true; auto. 
+          simpl. rewrite Heqt. reflexivity. 
+          
+          Qed.
+      
+        Theorem CWhile_congruence : forall t t' b b',
+            denote_expr t ≅ denote_expr t' ->
+            denote_imp b ≅ denote_imp b' ->
+            denote_imp (While t b) ≅ denote_imp (While t' b').
+      
+      
+        Proof.
+          intros t t' b b' Heqt Heqb.
+          simpl. unfold while.
+          eapply eq_itree_iter; intros ?? <-.
+          apply eqit_bind.
+          rewrite Heqt. reflexivity.
+      
+          intros []. case is_true; auto.
+          simpl. rewrite Heqb. reflexivity. reflexivity.
+          simpl. rewrite Heqb. reflexivity.
+          Qed.
+      
+       
+        Theorem CWhile_congruence_weak : forall t t' b b',
+            denote_expr t ≈ denote_expr t' ->
+            denote_imp b ≈ denote_imp b' ->
+            denote_imp (While t b) ≈ denote_imp (While t' b').
+        Proof.
+          intros t t' b b' Heqt Heqb.
+          simpl. unfold while.
+          apply eutt_iter' with (RI := eq). intros _ _ []. apply eutt_clo_bind with (UU := eq); try reflexivity.
+          assumption. intros. subst. destruct u2. simpl. reflexivity. simpl. rewrite Heqb. reflexivity. reflexivity.
+          Qed.
+          
+      
+      
+          Theorem denote_imp_fold_constants_stmt_with_congruence : forall s,
+              denote_imp (fold_constants_stmt s) ≅ denote_imp s.
+          Proof.
+            intros s; induction s.
+            - apply CAsgn_congruence. apply denote_imp_fold_constants_expr.
+            -  unfold fold_constants_stmt. fold fold_constants_stmt.
+               apply CSeq_congruence; try reflexivity.
+               apply IHs1. apply IHs2.
+            - unfold fold_constants_stmt. 
+              fold fold_constants_stmt.
+              unfold denote_imp. fold denote_imp.
+              rewrite <- (denote_imp_fold_constants_expr i).
+              destruct (fold_constants_expr i) eqn:eqi.
+              + apply CIf_congruence; try reflexivity. 
+                apply IHs1. apply IHs2.
+              + destruct v.
+                * simpl. rewrite bind_ret_l. simpl.  
+                  apply IHs2.
+                * simpl. rewrite bind_ret_l. simpl.  
+                  apply IHs1.
+              + apply CIf_congruence; try reflexivity.
+                apply IHs1. apply IHs2.
+              + apply CIf_congruence; try reflexivity.
+                apply IHs1. apply IHs2.
+              + apply CIf_congruence; try reflexivity.
+                apply IHs1. apply IHs2.
+            - unfold fold_constants_stmt. fold fold_constants_stmt.
+              unfold denote_imp. fold denote_imp.
+              unfold while.
+              setoid_rewrite <- (denote_imp_fold_constants_expr t).
+                destruct (fold_constants_expr t) eqn:eqt; 
+                try apply CWhile_congruence; try reflexivity; try apply IHs.
+                * destruct v. simpl.
+                  unfold iter. unfold Iter_Kleisli. unfold Basics.iter. unfold MonadIter_itree.
+                  rewrite unfold_iter. rewrite bind_bind.
+                  
+                  rewrite bind_ret_l. simpl. rewrite bind_ret_l. reflexivity.
+                  apply CWhile_congruence; try reflexivity. apply IHs.
+          - simpl.  reflexivity.
+            - reflexivity.
+          Qed.
+      
+          Theorem denote_imp_fold_constants_stmt_with_congruence_weak : forall s,
+              denote_imp (fold_constants_stmt s) ≈ denote_imp s.
+          Proof.
+            intros s; induction s.
+            - apply CAsgn_congruence_weak. apply denote_imp_fold_constants_expr_weak.
+            -  unfold fold_constants_stmt. fold fold_constants_stmt.
+               apply CSeq_congruence_weak; try reflexivity.
+               apply IHs1. apply IHs2.
+            - unfold fold_constants_stmt. 
+              fold fold_constants_stmt.
+              unfold denote_imp. fold denote_imp.
+              rewrite <- (denote_imp_fold_constants_expr_weak i).
+              destruct (fold_constants_expr i) eqn:eqi.
+              + apply CIf_congruence_weak; try reflexivity. 
+                apply IHs1. apply IHs2.
+              + destruct v.
+                * simpl. rewrite bind_ret_l. simpl.  
+                  apply IHs2.
+                * simpl. rewrite bind_ret_l. simpl.  
+                  apply IHs1.
+              + apply CIf_congruence_weak; try reflexivity.
+                apply IHs1. apply IHs2.
+              + apply CIf_congruence_weak; try reflexivity.
+                apply IHs1. apply IHs2.
+              + apply CIf_congruence_weak; try reflexivity.
+                apply IHs1. apply IHs2.
+            - unfold fold_constants_stmt. fold fold_constants_stmt.
+              unfold denote_imp. fold denote_imp.
+              unfold while.
+               
+              setoid_rewrite <- (denote_imp_fold_constants_expr_weak t).
+                destruct (fold_constants_expr t) eqn:eqt; 
+                try apply CWhile_congruence_weak; try reflexivity; try apply IHs.
+                * destruct v. simpl. rewrite unfold_iter_ktree. rewrite ? bind_ret_l. 
+                  now cbn; rewrite ? bind_ret_l.
+                  apply CWhile_congruence_weak; try reflexivity. apply IHs.
+          - simpl.  reflexivity. 
+            - reflexivity.
+              Qed.
+              
+      
+      
+  
+          
